src/crypto/aes/GCTR_s.fst
@@ -3,20 +3,19 @@ module GCTR_s
 open Types_s
 open FStar.Mul
 open AES_s
-open FStar.List.Tot.Base
+open FStar.Seq
 
-type gctr_plain = p:list quad32 { 256 * length p < nat32_max }
+// length plain < nat32_max / 256 <= spec max of 2**39 - 256;
+type gctr_plain = p:seq quad32 { 256 * length p < nat32_max }
 
 let inc32 (cb:quad32) (i:int) = 
   Quad32 ((cb.lo + i) % nat32_max) cb.mid_lo cb.mid_hi cb.hi
 
 let rec gctr_encrypt_recursive (icb:quad32) (plain:gctr_plain) 
-			       (alg:algorithm) (key:aes_key alg) (i:int) =
-  match plain with
-  | [] -> []
-  | hd :: tl -> (quad32_xor hd (aes_encrypt alg key (inc32 icb i))) :: (gctr_encrypt_recursive icb tl alg key (i + 1))
+			       (alg:algorithm) (key:aes_key alg) (i:int) : Tot (seq quad32) (decreases %[length plain]) =
+  if length plain = 0 then createEmpty
+  else cons (quad32_xor (head plain) (aes_encrypt alg key (inc32 icb i))) (gctr_encrypt_recursive icb (tail plain) alg key (i + 1))
   
-// length plain < nat32_max / 256 <= spec max of 2**39 - 256;
 let gctr_encrypt (icb:quad32) (plain:gctr_plain) (alg:algorithm) (key:aes_key alg) =
   gctr_encrypt_recursive icb plain alg key 0
   
